define an MST F* effect. worked surprisingly quickly. universe problems because of pre-condionality

experiments/dm4ms/TOTAL_MST.fst
@@ -7,7 +7,7 @@ open FStar.Tactics
 module W = FStar.Monotonic.Witnessed
 
 noeq type tstate = {
-  t: Type0;
+  t: Type u#a;
   rel: FStar.Preorder.preorder t;
 }
 
@@ -15,20 +15,20 @@ let stable (#state) (pred:state.t -> Type0) =
   forall h1 h2. (pred h1 /\ h1 `state.rel` h2) ==> pred h2
 
 noeq
-type free (state:tstate) (a:Type u#a) : Type u#(max 1 a) =
+type free (state:tstate u#b) (a:Type u#a) : Type u#(max 1 a b) =
 | Get : cont:(state.t -> free state a) -> free state a
 | Put : state.t -> cont:(unit -> free state a) -> free state a
 | Witness : p:(state.t -> Type0) -> cont:(unit -> free state a) -> free state a
 | Recall : p:(state.t -> Type0) -> cont:(unit -> free state a) -> free state a
 
-| PartialCall : (pre:pure_pre) -> cont:((squash pre) -> free u#a state a) -> free state a
+| PartialCall : (pre:pure_pre) -> cont:((squash pre) -> free state a) -> free state a
 | Return : a -> free state a
 
-let free_return (state:tstate) (a:Type) (x:a) : free state a =
+let free_return (state:tstate u#a) (a:Type u#b) (x:a) : free state a =
   Return x
 
 let rec free_bind
-  (state:tstate)
+  (state:tstate u#c)
   (a:Type u#a)
   (b:Type u#b)
   (l : free state a)
@@ -44,15 +44,15 @@ let rec free_bind
       PartialCall pre (fun _ ->
         free_bind state a b (fnc ()) k)
 
-let partial_call_wp (state:Type0) (pre:pure_pre) : st_wp_h state (squash pre) = 
+let partial_call_wp (state:tstate) (pre:pure_pre) : st_wp_h state.t (squash pre) = 
   fun p h0 -> pre /\ p () h0
 
-val theta : #a:Type u#a -> #state:tstate -> free state a -> st_wp_h state.t a
+val theta : #a:Type u#a -> #state:tstate u#c -> free state a -> st_wp_h state.t a
 let rec theta #a #state m =
   match m with
   | Return x -> st_return state.t _ x
   | PartialCall pre k ->
-      st_bind_wp state.t _ _ (partial_call_wp state.t pre) (fun r -> theta (k r))
+      st_bind_wp state.t _ _ (partial_call_wp state pre) (fun r -> theta (k r))
   | Get k ->
       st_bind_wp state.t _ _ (fun p h -> p h h) (fun r -> theta (k r))
   | Put h1 k ->
@@ -65,11 +65,13 @@ let rec theta #a #state m =
 let mst (state:tstate) (a:Type) (wp:st_wp_h state.t a)=
   m:(free state a){theta m ⊑ wp}
 
-let mst_return state (a:Type) (x:a) : mst state a (st_return state.t _ x) =
+#set-options "--print_universes"
+let mst_return (#state:tstate) (#a:Type) (x:a) : mst state a (st_return state.t _ x) =
   free_return state a x
 
+
 let mst_bind
-  (#state:tstate)
+  (#state:tstate u#c)
   (#a : Type u#a)
   (#b : Type u#b)
   (#wp_v : st_wp_h state.t a)
@@ -81,7 +83,7 @@ let mst_bind
   free_bind state a b v f
 
 let mst_subcomp
-  (#state:tstate)
+  (#state:tstate u#c)
   (#a : Type u#a)
   (#wp1 : st_wp_h state.t a)
   (#wp2 : st_wp_h state.t a)
@@ -90,7 +92,7 @@ let mst_subcomp
   Pure (mst state a wp2) (requires (wp1 ⊑ wp2)) (ensures (fun _ -> True)) =
   v
 
-let partial_return state (pre:pure_pre) : mst state (squash pre) (partial_call_wp state.t pre) =
+let partial_return state (pre:pure_pre) : mst state (squash pre) (partial_call_wp state pre) =
   PartialCall pre (Return)
 
 let get #state () : mst state state.t (fun p h0 -> p h0 h0) =
@@ -140,3 +142,146 @@ let test () : mst nat_state int (fun p h0 -> forall r h1. p r h1) =
         // put (h0+1) // TODO: can I revert the state to h0?
         // `mst_bind`
         // (fun () -> f ()))))
+
+
+
+
+open FStar.Monotonic.Heap
+
+let heap_state : tstate = { t = heap; rel = FStar.ST.heap_rel }
+
+let _stable (pred:heap_state.t -> Type0) = stable #heap_state pred
+
+let _mst a wp = mst heap_state a wp
+let _mst_bind a b wp_v wp_f v f = mst_bind #heap_state #a #b #wp_v #wp_f v f
+let _mst_return a x = mst_return #heap_state #a x
+
+let _mst_subcomp a wp1 wp2 v:
+  Pure (_mst a wp2) (requires (wp1 ⊑ wp2)) (ensures (fun _ -> True)) = mst_subcomp #heap_state #a #wp1 #wp2 v
+
+let mst_if_then_else (a : Type u#a)
+  (#wp1 : st_wp_h heap_state.t a)
+  (#wp2 : st_wp_h heap_state.t a)
+  (f : _mst a wp1) (g : _mst a wp2) (b : bool) : Type =
+  _mst a (st_if_then_else heap_state.t a b wp1 wp2)
+
+
+total
+reifiable
+reflectable
+effect {
+  STATEwp (a:Type) (wp : st_wp_h heap_state.t a)
+  with {
+       repr       = _mst
+     ; return     = _mst_return
+     ; bind       = _mst_bind
+     ; subcomp    = _mst_subcomp
+     ; if_then_else = mst_if_then_else
+     }
+}
+
+unfold
+let wp_lift_pure_st (w : pure_wp 'a) : st_wp_h heap_state.t 'a =
+  fun p h -> w (fun r -> p r h)
+
+val lift_pure_mst :
+  a: Type u#a ->
+  w: pure_wp a ->
+  f: (eqtype_as_type unit -> PURE a w) ->
+  Tot (_mst a (wp_lift_pure_st w))
+let lift_pure_mst a w f =
+  FStar.Monotonic.Pure.elim_pure_wp_monotonicity_forall ();
+  let lhs = partial_return heap_state (as_requires w) in
+  let rhs = (fun (pre:(squash (as_requires w))) -> _mst_return a (f pre)) in
+  let m = _mst_bind _ _ _ _ lhs rhs in
+  _mst_subcomp _ _ _ m
+
+sub_effect PURE ~> STATEwp = lift_pure_mst
+
+let _get () : STATEwp heap (fun p h -> p h h) = 
+  STATEwp?.reflect (get ())
+
+let _put (h1:heap) : STATEwp unit (fun p h0 -> (h0 `heap_state.rel` h1) /\ p () h1) = 
+  STATEwp?.reflect (put h1)
+
+
+(** *** START SECTION --- COPY PASTE FROM FStar.ST **)
+type heap_predicate = heap -> Type0
+
+[@@"opaque_to_smt"]
+let witnessed (p:heap_predicate{_stable p}) : Type0 = W.witnessed heap_state.rel p
+
+let _witness (pred:heap -> Type0) : STATEwp unit (fun p h -> pred h /\ _stable pred /\ (witnessed pred ==> p () h)) = 
+  STATEwp?.reflect (witness pred)
+
+let _recall (pred:heap_predicate{stable #heap_state pred}) : STATEwp unit (fun p h -> witnessed pred /\ (pred h ==> p () h)) = 
+  STATEwp?.reflect (recall pred)
+
+let st_pre           = st_pre_h heap
+let st_post' (a:Type) (pre:Type) = st_post_h' heap a pre
+let st_post  (a:Type) = st_post_h heap a
+let st_wp (a:Type)   = st_wp_h heap a
+
+effect ST (a:Type) (pre:st_pre) (post: (h:heap -> Tot (st_post' a (pre h)))) =
+  STATEwp a (fun (p:st_post a) (h:heap) -> pre h /\ (forall a h1. post h a h1 ==> p a h1))
+effect St (a:Type) = ST a (fun h -> True) (fun h0 r h1 -> True)
+
+
+let contains_pred (#a:Type) (#rel:FStar.Preorder.preorder a) (r:mref a rel) = fun h -> h `contains` r
+
+type mref (a:Type0) (rel:FStar.Preorder.preorder a) =
+  r:Heap.mref a rel{is_mm r = false /\ witnessed (contains_pred r)}
+
+let alloc (#a:Type) (#rel:FStar.Preorder.preorder a) (init:a)
+  :ST (mref a rel)
+      (fun h -> True)
+      (fun h0 r h1 -> fresh r h0 h1 /\ modifies Set.empty h0 h1 /\ sel h1 r == init)
+  = let h0 = _get () in
+    let r, h1 = alloc rel h0 init false in
+    _put h1;
+    _witness (contains_pred r);
+    r
+
+let read (#a:Type) (#rel:FStar.Preorder.preorder a) (r:mref a rel) :STATEwp a (fun p h -> p (sel h r) h)
+  = let h0 = _get () in
+    assert (_stable (contains_pred r));
+    _recall (contains_pred r);
+    Heap.lemma_sel_equals_sel_tot_for_contained_refs h0 r;
+    sel_tot h0 r
+
+let write (#a:Type) (#rel:FStar.Preorder.preorder a) (r:mref a rel) (v:a)
+  : ST unit
+    (fun h -> rel (sel h r) v)
+    (fun h0 x h1 -> rel (sel h0 r) v /\ h0 `contains` r /\
+                 modifies (Set.singleton (addr_of r)) h0 h1 /\ equal_dom h0 h1 /\
+                 sel h1 r == v)
+  = let h0 = _get () in
+    assert (_stable (contains_pred r));
+    _recall (contains_pred r);
+    let h1 = upd_tot h0 r v in
+    Heap.lemma_distinct_addrs_distinct_preorders ();
+    Heap.lemma_distinct_addrs_distinct_mm ();
+    Heap.lemma_upd_equals_upd_tot_for_contained_refs h0 r v;
+    _put h1
+
+let op_Bang (#a:Type) (#rel:FStar.Preorder.preorder a) (r:mref a rel)
+  : STATEwp a (fun p h -> p (sel h r) h)
+= read #a #rel r
+
+let op_Colon_Equals (#a:Type) (#rel:FStar.Preorder.preorder a) (r:mref a rel) (v:a)
+  : ST unit
+    (fun h -> rel (sel h r) v)
+    (fun h0 x h1 -> rel (sel h0 r) v /\ h0 `contains` r /\
+                 modifies (Set.singleton (addr_of r)) h0 h1 /\ equal_dom h0 h1 /\
+                 sel h1 r == v)
+= write #a #rel r v
+
+type ref (a:Type0) = mref a (FStar.Heap.trivial_preorder a)
+(** *** END SECTION --- COPY PASTE FROM FStar.ST **)
+
+let landins_knot_fs () : St nat = 
+  let id : nat -> St nat = fun x -> x in
+  let r : ref (nat -> St nat) = alloc id in (** because of pre-conditionality, we cannot even put arrows in the heap *)
+  // let f : nat -> St nat = (fun x -> !r x) in
+  // r := f;
+  f 0
